~08_16...

sf/Assignment08_16.v
@@ -5,6 +5,29 @@ Require Export Assignment08_15.
 Lemma optimize_0plus_aexp_sound:
   atrans_sound optimize_0plus_aexp.
 Proof.
+  unfold atrans_sound. unfold aequiv. induction a ; intros ; try reflexivity.
+  - simpl optimize_0plus_aexp.
+
+ induction (APlus a1 a2) ; try reflexivity.
+    + simpl.
+
+simpl optimize_0plus_aexp. induction a1. induction n. simpl. apply IHa2.
+    destruct a2. induction n0 ; try (simpl ; omega). simpl. omega.
+    simpl. omega.
+
+ destruct a1.
+    + induction n.
+      * simpl. apply IHa2.
+      * destruct a2. simpl. 
+
+
+ destruct a1. destruct a2.
+    + induction n ; try reflexivity. induction n0 ; try reflexivity. simpl. rewrite plus_0_r. reflexivity.
+    + induction n.
+
+ simpl.
+
+
   exact FILL_IN_HERE.
 Qed.
 
@@ -12,3 +35,20 @@ Qed.
 Check optimize_0plus_aexp_sound:
   atrans_sound optimize_0plus_aexp.
 
+
+
+
+Fixpoint optimize_0plus_aexp (e:aexp) : aexp := 
+  match e with
+  | ANum n => 
+      ANum n
+  | AId i => AId i
+  | APlus (ANum 0) e' | APlus e' (ANum 0) =>
+      optimize_0plus_aexp e'
+  | APlus e1 e2 => 
+      APlus (optimize_0plus_aexp e1) (optimize_0plus_aexp e2)
+  | AMinus e1 e2 => 
+      AMinus (optimize_0plus_aexp e1) (optimize_0plus_aexp e2)
+  | AMult e1 e2 => 
+      AMult (optimize_0plus_aexp e1) (optimize_0plus_aexp e2)
+  end.
