sf/Assignment08_12.v
@@ -7,11 +7,13 @@ Theorem CSeq_congruence : forall c1 c1' c2 c2',
   cequiv c1 c1' -> cequiv c2 c2' ->
   cequiv (c1;;c2) (c1';;c2').
 Proof. 
-  exact FILL_IN_HERE.
+  unfold cequiv. intros. split ; intros ; inversion H1 ; subst ; apply H in H4 ; apply H0 in H7 ;
+  apply E_Seq with (st' := st'0) ; assumption ; assumption.
 Qed.
 
 (*-- Check --*)
 Check CSeq_congruence : forall c1 c1' c2 c2',
   cequiv c1 c1' -> cequiv c2 c2' ->
   cequiv (c1;;c2) (c1';;c2').
+
 
