sf/Assignment08_13.v
@@ -7,7 +7,17 @@ Theorem CIf_congruence : forall b b' c1 c1' c2 c2',
   bequiv b b' -> cequiv c1 c1' -> cequiv c2 c2' ->
   cequiv (IFB b THEN c1 ELSE c2 FI) (IFB b' THEN c1' ELSE c2' FI).
 Proof.
-  exact FILL_IN_HERE.
+  unfold bequiv, cequiv. intros. split ; subst.
+  - destruct (beval st b) eqn: H2 ; subst.
+    + intros. apply E_IfTrue. rewrite <- H2. symmetry. apply H. inversion H3 ; subst.
+      apply H0 in H10. assumption. rewrite H2 in H9. inversion H9.
+    + intros. apply E_IfFalse. rewrite <- H2. symmetry. apply H. inversion H3 ; subst.
+      rewrite H2 in H9. inversion H9. apply H1 in H10. assumption.
+  - destruct (beval st b') eqn: H2; subst.
+    + intros. apply E_IfTrue. rewrite <- H2. apply H. inversion H3 ; subst.
+      apply H0 in H10. assumption. rewrite H2 in H9. inversion H9.
+    + intros. apply E_IfFalse. rewrite <- H2. apply H. inversion H3 ; subst.
+      rewrite H2 in H9. inversion H9. apply H1 in H10. assumption.
 Qed.
 
 (*-- Check --*)
