sf/Assignment08_15.v
@@ -2,6 +2,21 @@ Require Export Assignment08_14.
 
 (* problem #15: 10 points *)
 
+Lemma WHILE_true_nonterm : forall b c st st',
+     bequiv b BTrue ->
+     ~( (WHILE b DO c END) / st || st' ).
+Proof. 
+  intros b c st st' Hb.
+  intros H.
+  remember (WHILE b DO c END) as cw eqn:Heqcw.
+  ceval_cases (induction H) Case;
+    inversion Heqcw; subst; clear Heqcw.
+  Case "E_WhileEnd". 
+    unfold bequiv in Hb.
+    rewrite Hb in H. inversion H.
+  Case "E_WhileLoop". 
+    apply IHceval2. reflexivity.  Qed.
+
 (** **** Exercise: 3 stars (fold_constants_com_sound)  *)
 (** Complete the [WHILE] case of the following proof. *)
 
@@ -26,13 +41,22 @@ Proof.
          is easy to prove from the IH and fold_constants_bexp_sound *)
       try (apply CIf_congruence; assumption).
     SCase "b always true".
-      apply trans_cequiv with c1; try assumption.
+      apply trans_cequiv with c1 ; try assumption.
       apply IFB_true; assumption.
     SCase "b always false".
       apply trans_cequiv with c2; try assumption.
       apply IFB_false; assumption.
   Case "WHILE".
-    exact FILL_IN_HERE.
+    { assert (bequiv b (fold_constants_bexp b)). apply fold_constants_bexp_sound.
+      destruct (fold_constants_bexp b) eqn: Hb ; try (apply CWhile_congruence ; assumption).
+      - unfold cequiv. split ; intros. 
+        + apply WHILE_true_nonterm with b c st st' in H. apply H in H0. inversion H0.
+        + apply loop_never_stops in H0. inversion H0.
+      - unfold cequiv. split ; intros.
+        + inversion H0 ; subst. apply E_Skip. apply WHILE_true_nonterm with b c st'0 st' in H7.
+          inversion H7. unfold bequiv in H. simpl in H. rewrite H in H3. inversion H3.
+        + inversion H0 ; subst. apply E_WhileEnd. apply H.
+    }
 Qed.
 
 (*-- Check --*)
